cedar-lean/Cedar/Thm/Validation/Typechecker/BinaryApp/Arith.lean
@@ -60,7 +60,7 @@ theorem type_of_int_arith_is_sound {op₂ : BinaryOp} {x₁ x₂ : Expr} {c₁ c
   (ih₁ : TypeOfIsSound x₁)
   (ih₂ : TypeOfIsSound x₂) :
   GuardedCapabilitiesInvariant (Expr.binaryApp op₂ x₁ x₂) c₂ request entities ∧
-  ∃ v, EvaluatesTo (Expr.binaryApp op₂ x₁ x₂) request entities v ∧ InstanceOfType v ty.typeOf
+  ∃ v, EvaluatesTo (Expr.binaryApp op₂ x₁ x₂) request entities v ∧ InstanceOfType env v ty.typeOf
 := by
   have ⟨hc, hty, ht₁, ht₂⟩ := type_of_int_arith_inversion h₀ h₃
   subst hc ; rw [hty]
