cedar-lean/Cedar/Thm/Validation/Typechecker/BinaryApp/Contains.lean
@@ -58,7 +58,7 @@ theorem type_of_contains_is_sound {x₁ x₂ : Expr} {c₁ c₂ : Capabilities} 
   (ih₁ : TypeOfIsSound x₁)
   (ih₂ : TypeOfIsSound x₂) :
   GuardedCapabilitiesInvariant (Expr.binaryApp .contains x₁ x₂) c₂ request entities ∧
-  ∃ v, EvaluatesTo (Expr.binaryApp .contains x₁ x₂) request entities v ∧ InstanceOfType v ty.typeOf
+  ∃ v, EvaluatesTo (Expr.binaryApp .contains x₁ x₂) request entities v ∧ InstanceOfType env v ty.typeOf
 := by
   have ⟨hc, hty, ty₁, ty₂, _, ht₁, ht₂⟩ := type_of_contains_inversion h₃
   subst hc ; rw [hty]
