cedar-lean/Cedar/Thm/Validation/Typechecker/Call.lean
@@ -98,7 +98,7 @@ theorem type_of_call_decimal_inversion {xs : List Expr} {c c' : Capabilities} {e
 theorem type_of_call_decimal_is_sound {xs : List Expr} {c₁ c₂ : Capabilities} {env : Environment} {ty : TypedExpr} {request : Request} {entities : Entities}
   (h₁ : typeOf (Expr.call .decimal xs) c₁ env = Except.ok (ty, c₂)) :
   GuardedCapabilitiesInvariant (Expr.call .decimal xs) c₂ request entities ∧
-  ∃ v, EvaluatesTo (Expr.call .decimal xs) request entities v ∧ InstanceOfType v ty.typeOf
+  ∃ v, EvaluatesTo (Expr.call .decimal xs) request entities v ∧ InstanceOfType env v ty.typeOf
 := by
   have ⟨h₂, h₃, s, h₄, h₅⟩ := type_of_call_decimal_inversion h₁
   rw [h₂]
@@ -137,7 +137,7 @@ theorem type_of_call_datetime_inversion {xs : List Expr} {c c' : Capabilities} {
 theorem type_of_call_datetime_is_sound {xs : List Expr} {c₁ c₂ : Capabilities} {env : Environment} {ty : TypedExpr} {request : Request} {entities : Entities}
   (h₁ : typeOf (Expr.call .datetime xs) c₁ env = Except.ok (ty, c₂)) :
   GuardedCapabilitiesInvariant (Expr.call .datetime xs) c₂ request entities ∧
-  ∃ v, EvaluatesTo (Expr.call .datetime xs) request entities v ∧ InstanceOfType v ty.typeOf
+  ∃ v, EvaluatesTo (Expr.call .datetime xs) request entities v ∧ InstanceOfType env v ty.typeOf
 := by
   have ⟨h₂, h₃, s, h₄, h₅⟩ := type_of_call_datetime_inversion h₁
   rw [h₂]
@@ -174,7 +174,7 @@ theorem type_of_call_duration_inversion {xs : List Expr} {c c' : Capabilities} {
 theorem type_of_call_duration_is_sound {xs : List Expr} {c₁ c₂ : Capabilities} {env : Environment} {ty : TypedExpr} {request : Request} {entities : Entities}
   (h₁ : typeOf (Expr.call .duration xs) c₁ env = Except.ok (ty, c₂)) :
   GuardedCapabilitiesInvariant (Expr.call .duration xs) c₂ request entities ∧
-  ∃ v, EvaluatesTo (Expr.call .duration xs) request entities v ∧ InstanceOfType v ty.typeOf
+  ∃ v, EvaluatesTo (Expr.call .duration xs) request entities v ∧ InstanceOfType env v ty.typeOf
 := by
   have ⟨h₂, h₃, s, h₄, h₅⟩ := type_of_call_duration_inversion h₁
   rw [h₂]
@@ -212,7 +212,7 @@ theorem type_of_call_ip_inversion {xs : List Expr} {c c' : Capabilities} {env : 
 theorem type_of_call_ip_is_sound {xs : List Expr} {c₁ c₂ : Capabilities} {env : Environment} {ty : TypedExpr} {request : Request} {entities : Entities}
   (h₁ : typeOf (Expr.call .ip xs) c₁ env = Except.ok (ty, c₂)) :
   GuardedCapabilitiesInvariant (Expr.call .ip xs) c₂ request entities ∧
-  ∃ v, EvaluatesTo (Expr.call .ip xs) request entities v ∧ InstanceOfType v ty.typeOf
+  ∃ v, EvaluatesTo (Expr.call .ip xs) request entities v ∧ InstanceOfType env v ty.typeOf
 := by
   have ⟨h₂, h₃, s, h₄, h₅⟩ := type_of_call_ip_inversion h₁
   rw [h₂]
@@ -322,7 +322,7 @@ theorem type_of_call_decimal_comparator_is_sound {xfn : ExtFun} {xs : List Expr}
   (h₃ : typeOf (Expr.call xfn xs) c₁ env = Except.ok (ty, c₂))
   (ih : ∀ (xᵢ : Expr), xᵢ ∈ xs → TypeOfIsSound xᵢ) :
   GuardedCapabilitiesInvariant (Expr.call xfn xs) c₂ request entities ∧
-  ∃ v, EvaluatesTo (Expr.call xfn xs) request entities v ∧ InstanceOfType v ty.typeOf
+  ∃ v, EvaluatesTo (Expr.call xfn xs) request entities v ∧ InstanceOfType env v ty.typeOf
 := by
   have ⟨h₄, h₅, x₁, x₂, c₁', c₂', h₆, h₇, h₈⟩ := type_of_call_decimal_comparator_inversion h₀ h₃
   rw [h₄]
@@ -395,7 +395,7 @@ theorem type_of_call_isInRange_comparator_is_sound {xs : List Expr} {c₁ c₂ :
   (h₃ : typeOf (Expr.call .isInRange xs) c₁ env = Except.ok (ty, c₂))
   (ih : ∀ (xᵢ : Expr), xᵢ ∈ xs → TypeOfIsSound xᵢ) :
   GuardedCapabilitiesInvariant (Expr.call .isInRange xs) c₂ request entities ∧
-  ∃ v, EvaluatesTo (Expr.call .isInRange xs) request entities v ∧ InstanceOfType v ty.typeOf
+  ∃ v, EvaluatesTo (Expr.call .isInRange xs) request entities v ∧ InstanceOfType env v ty.typeOf
 := by
   have ⟨h₄, h₅, x₁, x₂, c₁', c₂', h₆, h₇, h₈⟩ := type_of_call_isInRange_inversion h₃
   rw [h₄]
@@ -503,7 +503,7 @@ theorem type_of_call_toTime_is_sound {xs : List Expr} {c₁ c₂ : Capabilities}
   (h₃ : typeOf (Expr.call .toTime xs) c₁ env = Except.ok (ty, c₂))
   (ih : ∀ (xᵢ : Expr), xᵢ ∈ xs → TypeOfIsSound xᵢ) :
   GuardedCapabilitiesInvariant (Expr.call .toTime xs) c₂ request entities ∧
-  ∃ v, EvaluatesTo (Expr.call .toTime xs) request entities v ∧ InstanceOfType v ty.typeOf
+  ∃ v, EvaluatesTo (Expr.call .toTime xs) request entities v ∧ InstanceOfType env v ty.typeOf
 := by
   have ⟨h₄, h₅, x₁, c₁', h₆, h₇⟩ := type_of_call_toTime_inversion h₃
   rw [h₄]
@@ -563,7 +563,7 @@ theorem type_of_call_toDate_is_sound {xs : List Expr} {c₁ c₂ : Capabilities}
   (h₃ : typeOf (Expr.call .toDate xs) c₁ env = Except.ok (ty, c₂))
   (ih : ∀ (xᵢ : Expr), xᵢ ∈ xs → TypeOfIsSound xᵢ) :
   GuardedCapabilitiesInvariant (Expr.call .toDate xs) c₂ request entities ∧
-  ∃ v, EvaluatesTo (Expr.call .toDate xs) request entities v ∧ InstanceOfType v ty.typeOf
+  ∃ v, EvaluatesTo (Expr.call .toDate xs) request entities v ∧ InstanceOfType env v ty.typeOf
 := by
   have ⟨h₄, h₅, x₁, c₁', h₆, h₇⟩ := type_of_call_toDate_inversion h₃
   rw [h₄]
@@ -633,7 +633,7 @@ theorem type_of_call_offset_is_sound {xs : List Expr} {c₁ c₂ : Capabilities}
   (h₃ : typeOf (Expr.call .offset xs) c₁ env = Except.ok (ty, c₂))
   (ih : ∀ (xᵢ : Expr), xᵢ ∈ xs → TypeOfIsSound xᵢ) :
   GuardedCapabilitiesInvariant (Expr.call .offset xs) c₂ request entities ∧
-  ∃ v, EvaluatesTo (Expr.call .offset xs) request entities v ∧ InstanceOfType v ty.typeOf
+  ∃ v, EvaluatesTo (Expr.call .offset xs) request entities v ∧ InstanceOfType env v ty.typeOf
 := by
     have ⟨h₄, h₅, x₁, x₂, c₁', c₂', h₆, h₇, h₈⟩ := type_of_call_offset_inversion h₃
     rw [h₄]
@@ -714,7 +714,7 @@ theorem type_of_call_durationSince_is_sound {xs : List Expr} {c₁ c₂ : Capabi
   (h₃ : typeOf (Expr.call .durationSince xs) c₁ env = Except.ok (ty, c₂))
   (ih : ∀ (xᵢ : Expr), xᵢ ∈ xs → TypeOfIsSound xᵢ) :
   GuardedCapabilitiesInvariant (Expr.call .durationSince xs) c₂ request entities ∧
-  ∃ v, EvaluatesTo (Expr.call .durationSince xs) request entities v ∧ InstanceOfType v ty.typeOf
+  ∃ v, EvaluatesTo (Expr.call .durationSince xs) request entities v ∧ InstanceOfType env v ty.typeOf
 := by
     have ⟨h₄, h₅, x₁, x₂, c₁', c₂', h₆, h₇, h₈⟩ := type_of_call_durationSince_inversion h₃
     rw [h₄]
@@ -795,7 +795,7 @@ theorem type_of_call_ipAddr_recognizer_is_sound {xfn : ExtFun} {xs : List Expr} 
   (h₃ : typeOf (Expr.call xfn xs) c₁ env = Except.ok (ty, c₂))
   (ih : ∀ (xᵢ : Expr), xᵢ ∈ xs → TypeOfIsSound xᵢ) :
   GuardedCapabilitiesInvariant (Expr.call xfn xs) c₂ request entities ∧
-  ∃ v, EvaluatesTo (Expr.call xfn xs) request entities v ∧ InstanceOfType v ty.typeOf
+  ∃ v, EvaluatesTo (Expr.call xfn xs) request entities v ∧ InstanceOfType env v ty.typeOf
 := by
   have ⟨h₄, h₅, x₁, c₁', h₆, h₇⟩ := type_of_call_ipAddr_recognizer_inversion h₀ h₃
   rw [h₄]
@@ -868,7 +868,7 @@ theorem type_of_call_duration_converter_is_sound {xfn : ExtFun} {xs : List Expr}
   (h₃ : typeOf (Expr.call xfn xs) c₁ env = Except.ok (ty, c₂))
   (ih : ∀ (xᵢ : Expr), xᵢ ∈ xs → TypeOfIsSound xᵢ) :
   GuardedCapabilitiesInvariant (Expr.call xfn xs) c₂ request entities ∧
-  ∃ v, EvaluatesTo (Expr.call xfn xs) request entities v ∧ InstanceOfType v ty.typeOf
+  ∃ v, EvaluatesTo (Expr.call xfn xs) request entities v ∧ InstanceOfType env v ty.typeOf
 := by
   have ⟨h₄, h₅, x₁, c₁', h₆, h₇⟩ := type_of_call_duration_converter_inversion h₀ h₃
   rw [h₄]
@@ -900,7 +900,7 @@ theorem type_of_call_is_sound {xfn : ExtFun} {xs : List Expr} {c₁ c₂ : Capab
   (h₃ : typeOf (Expr.call xfn xs) c₁ env = Except.ok (ty, c₂))
   (ih : ∀ (xᵢ : Expr), xᵢ ∈ xs → TypeOfIsSound xᵢ) :
   GuardedCapabilitiesInvariant (Expr.call xfn xs) c₂ request entities ∧
-  ∃ v, EvaluatesTo (Expr.call xfn xs) request entities v ∧ InstanceOfType v ty.typeOf
+  ∃ v, EvaluatesTo (Expr.call xfn xs) request entities v ∧ InstanceOfType env v ty.typeOf
 := by
   match xfn with
   | .decimal            => exact type_of_call_decimal_is_sound h₃
