cedar-lean/Cedar/Thm/Validation/Typechecker/Set.lean
@@ -232,7 +232,7 @@ theorem type_of_set_is_sound_ok { xs : List Expr } { c₁ : Capabilities } { env
   (h₃ : ∀ (xᵢ : Expr), xᵢ ∈ xs → ∃ txᵢ cᵢ, (typeOf xᵢ c₁ env) = Except.ok (txᵢ, cᵢ) ∧ (txᵢ.typeOf ⊔ ty) = some ty)
   (h₄ : (xs.mapM fun x => evaluate x request entities) = Except.ok vs)
   (h₅ : v ∈ vs):
-  InstanceOfType v ty
+  InstanceOfType env v ty
 := by
   cases xs
   case nil =>
@@ -277,7 +277,7 @@ theorem type_of_set_is_sound {xs : List Expr} {c₁ c₂ : Capabilities} {env : 
   (h₃ : typeOf (Expr.set xs) c₁ env = Except.ok (sty, c₂))
   (ih : ∀ (xᵢ : Expr), xᵢ ∈ xs → TypeOfIsSound xᵢ) :
   GuardedCapabilitiesInvariant (Expr.set xs) c₂ request entities ∧
-  ∃ v, EvaluatesTo (Expr.set xs) request entities v ∧ InstanceOfType v sty.typeOf
+  ∃ v, EvaluatesTo (Expr.set xs) request entities v ∧ InstanceOfType env v sty.typeOf
 := by
   have ⟨h₆, txs, ty, h₄, h₅⟩ := type_of_set_inversion h₃
   subst h₆ ; rw [h₄]
